WIP

mem/Mem0.v
@@ -5,6 +5,7 @@ Require Import STS.
 Require Import Behavior.
 Require Import Mod ModSem SimModSem ModSemFacts.
 Require Import Skeleton.
+Require Import SimModSemStrong.
 
 Set Implicit Arguments.
 Set Typeclasses Depth 5.
@@ -12,6 +13,12 @@ Set Typeclasses Depth 5.
 
 
 
+Ltac my_steps :=
+  repeat (esplits; my_red_both;
+          try (guclo sim_itree_indC_spec; first [apply sim_itree_indC_choose_tgt|apply sim_itree_indC_take_src|econs]; et);
+          try (gstep; eapply sim_itree_pput; eauto);
+          try (gstep; eapply sim_itree_pget; eauto);
+          i; des; ss; subst; et).
 
 Section PROOF.
 
@@ -110,18 +117,10 @@ Section PROOF.
     - eapply NAME in Heq0; ss. congruence.
   Qed.
 
-  Program Definition Mem: Mod.t := {|
-    Mod.get_modsem := MemSem;
-    Mod.sk := Sk.unit;
-  |}
-  .
-  Next Obligation.
-    ii. r in EQV. unfold MemSem. ss. f_equiv.
-    f_equiv. erewrite equiv_load_mem; ss.
-  Qed.
-  Next Obligation.
-    i; cbn.
-    eapply ModSemPair.adequacy. ss.
+  Lemma affine_aux: ∀ sk0 sk1 (EQV: Sk.extends sk0 sk1) (WF: Sk.wf sk1),
+      ModSemPair.sim (MemSem sk0) (MemSem sk1).
+  Proof.
+    i. ss.
     econs.
     { instantiate (1:=top2). ss. }
     2: { instantiate (2:=unit).
@@ -228,6 +227,201 @@ Section PROOF.
         bsimpl; des; des_sumbool; ss; subst; exploit W; et; i; try congruence.
       - clear Heq2. exploit W; et; i; try congruence.
       - clear Heq2. exploit W; et; i; try congruence.
+    }
+  Qed.
+
+  Lemma sim_strong_bar: ∀ a b, ModSemPair.sim a b -> ModSemPair.sim ( |a| ) ( |b| ).
+  Proof.
+    i. upt. des_ifs; ss. inv H.
+    unshelve econs; et.
+    i. unfold bar, ModSem.bar in FINDS. ss. rewrite in_map_iff in *. des.
+    destruct x; ss. clarify.
+    hexploit sim_fnsems; et. intro T; des.
+    esplits; et.
+    { rewrite in_map_iff. esplits; et. ss. }
+    clear - SIM. ii. subst. exploit SIM; et. instantiate (1:=y). intro T.
+    unfold bar, ktree_Bar, bar, itree_Bar.
+    abstr (i y) i_src.
+    abstr (f_tgt y) i_tgt.
+    clear_tac.
+    revert T.
+    clear Heqitr_src. 
+    ss.
+  Qed.
+
+  Fixpoint sim_str (n: nat): ModSem.t -> ModSem.t -> Prop :=
+    match n with
+    | 0 => λ a b, ModSemPair.sim a b
+    | S n => λ a b, sim_str n ( |a| ) ( |b| ) ∧ ∀ s, sim_str n (𝑤_{s} a) (𝑤_{s} b)
+    end
+  .
+
+  Lemma sim_str_intro
+    (IHB: ∀ a b, ModSemPair.sim a b -> ModSemPair.sim ( |a| ) ( |b| ))
+    (IHW: ∀ a b, ModSemPair.sim a b -> ∀ s, ModSemPair.sim ( 𝑤_{s} a ) ( 𝑤_{s} b ))
+    a b
+    (BASE: ModSemPair.sim a b)
+    :
+    ∀ n, sim_str n a b.
+  Proof.
+    i. gen a b. induction n; i; ss.
+    esplits; et.
+  Qed.
+
+  Lemma sim_str_ref_str: ∀ a b, (∀ n, sim_str n a b) -> b ⊑S a.
+  Proof.
+    ii. gen a b. induction n; i; ss.
+    { eapply ModSemPair.adequacy; et. eapply (H 0). }
+    esplits; et.
+    - eapply IHn; et. i. specialize (H (S n0)). ss. des; et.
+    - i. eapply IHn; et. i. specialize (H (S n0)). ss. des; et.
+  Qed.
+
+  Local Opaque MemSem.
+  Lemma affine_aux2: ∀ n, ∀ sk0 sk1 (EQV: Sk.extends sk0 sk1) (WF: Sk.wf sk1),
+      sim_str n (MemSem sk0) (MemSem sk1).
+  Proof.
+    induction n; i.
+    { eapply affine_aux; et. }
+    ss. esplits; ss.
+    admit "tt".
+    admit "tt".
+  Qed.
+  Local Transparent MemSem.
+
+
+
+  Program Definition Mem: Mod.t := {|
+    Mod.get_modsem := MemSem;
+    Mod.sk := Sk.unit;
+  |}
+  .
+  Next Obligation.
+    ii. r in EQV. unfold MemSem. ss. f_equiv.
+    f_equiv. erewrite equiv_load_mem; ss.
+  Qed.
+  Next Obligation.
+    i. eapply sim_str_ref_str. i.
+    i; cbn.
+    ii. induction n.
+    { eapply ModSemPair.adequacy.
+      eapply affine_aux; ss.
+    }
+    Local Opaque MemSem.
+    ss.
+    split; ss.
+    -
+      ss.
+    econs.
+    { instantiate (1:=top2). ss. }
+    2: { instantiate (2:=unit).
+         instantiate (1:=fun _ '(st_src, st_tgt) =>
+                           exists m0 m1, st_tgt = Any.upcast m0 /\ st_src = Any.upcast m1 /\ mem_extends m1 m0).
+         ss. esplits; ss; et.
+         r. esplits; ss. i. uo. des_ifs_safe.
+         rr in EQV. des. rr in EQV. unfold oplus, Sk.add in *. ss. rr in WF.
+         erewrite alist_permutation_find.
+         2: { et. }
+         2: { sym; et. }
+         erewrite alist_find_app; et. ss.
+    }
+    ss. ii. des; ss; clarify.
+    {
+      esplits; ss; et. ii. des; subst.
+      rr in SIMMRS1. des.
+      eapply sim_itree_fsubset with []; ss.
+      unfold cfunU, allocF.
+      ginit. my_steps.
+      destruct (Any.downcast y) eqn:T.
+      2: { cbn. unfold triggerUB. my_steps. }
+      my_steps. des_ifs; my_steps; unfold triggerUB; my_steps.
+      destruct v; my_steps; des_ifs; my_steps; unfold triggerUB; my_steps.
+      rr. esplits; ss; et.
+      2: { rewrite NB; ss. }
+      rr. ss. esplits; try lia.
+      - ii. rewrite NB in *. unfold update in *. des_ifs; ss; et.
+      - ii. rewrite NB in *. unfold update in *. des_ifs; ss; et.
+    }
+    {
+      esplits; ss; et. ii. des; subst.
+      rr in SIMMRS1. des.
+      eapply sim_itree_fsubset with []; ss.
+      unfold cfunU, freeF.
+      ginit. my_steps.
+      destruct (Any.downcast y) eqn:T.
+      2: { cbn. unfold triggerUB. my_steps. }
+      my_steps. des_ifs; my_steps; unfold triggerUB; my_steps.
+      destruct v; my_steps; des_ifs; my_steps; unfold triggerUB; my_steps.
+      destruct blk; my_steps; des_ifs; my_steps; unfold triggerUB; my_steps.
+      destruct (Mem.free m1 n ofs) eqn:U.
+      2: { cbn. unfold triggerUB. my_steps. }
+      my_steps.
+      unfold Mem.free in *. des_ifs_safe. rewrite <- BLK. des_ifs. my_steps.
+      rr. esplits; ss; et.
+      rr. ss. esplits; try lia.
+      - ii. unfold update in *. des_ifs; ss; et.
+      - ii. unfold update in *. des_ifs; ss; et.
+    }
+    {
+      esplits; ss; et. ii. des; subst.
+      rr in SIMMRS1. des.
+      eapply sim_itree_fsubset with []; ss.
+      unfold cfunU, loadF.
+      ginit. my_steps.
+      destruct (Any.downcast y) eqn:T.
+      2: { cbn. unfold triggerUB. my_steps. }
+      my_steps. des_ifs; my_steps; unfold triggerUB; my_steps.
+      destruct v; my_steps; des_ifs; my_steps; unfold triggerUB; my_steps.
+      destruct (Mem.load m1 blk ofs) eqn:U.
+      2: { cbn. unfold triggerUB. my_steps. }
+      my_steps.
+      assert(V: Mem.load m0 blk ofs = Some v).
+      { destruct blk; ss; et. rewrite <- BLK; et. }
+      rewrite V; ss. my_steps.
+      rr. esplits; ss; et.
+    }
+    {
+      esplits; ss; et. ii. des; subst.
+      rr in SIMMRS1. des.
+      eapply sim_itree_fsubset with []; ss.
+      unfold cfunU, storeF.
+      ginit. my_steps.
+      destruct (Any.downcast y) eqn:T.
+      2: { cbn. unfold triggerUB. my_steps. }
+      my_steps. des_ifs; my_steps; unfold triggerUB; my_steps.
+      destruct v; my_steps; des_ifs; my_steps; unfold triggerUB; my_steps.
+      destruct (Mem.store m1 blk ofs) eqn:U.
+      2: { cbn. unfold triggerUB. my_steps. }
+      my_steps.
+      unfold Mem.store in *. des_ifs_safe.
+      assert(U: Mem.cnts m0 blk ofs = Some v).
+      { destruct blk; ss; et. rewrite <- BLK; et. }
+      des_ifs. my_steps.
+      rr. esplits; ss; et.
+      rr. ss. esplits; try lia.
+      - ii. extensionalities ofs0. rewrite BLK; ss.
+      - ii. des_ifs; ss; et.
+    }
+    {
+      esplits; ss; eauto 10. ii. des; subst.
+      assert(W:=extends_valid_ptr SIMMRS1).
+      rr in SIMMRS1. des.
+      eapply sim_itree_fsubset with []; ss.
+      unfold cfunU, cmpF.
+      ginit. my_steps.
+      destruct (Any.downcast y) eqn:T.
+      2: { cbn. unfold triggerUB. my_steps. }
+      my_steps. des_ifs; my_steps; unfold triggerUB; my_steps.
+      destruct (vcmp m1 v v0) eqn:U.
+      2: { cbn. unfold triggerUB. my_steps. }
+      unfold vcmp in *. des_ifs; my_steps; des_ifs; my_steps; rr; esplits; ss;
+        bsimpl; des; des_sumbool; ss; subst; exploit W; et; i; try congruence.
+      - clear Heq2. exploit W; et; i; try congruence.
+      - clear Heq2. exploit W; et; i; try congruence.
+    }
+    }
+    {
+      ss.
     }
   Qed.
   Next Obligation.
