ems/ModSem.v
@@ -448,11 +448,11 @@ Section MODSEM.
 
 
 
-  Global Instance refs: RefStrong _t :=
-    fun ms0 ms1 => Forall2 (fun '(fn0, ktr0) '(fn1, ktr1) => fn0 = fn1 /\
-                       (forall x, simg (fun _ _ => eq) 0 0 (ktr0 x) (ktr1 x)))
-                     ms0.(fnsems) ms1.(fnsems)
-                   /\ ms0.(initial_st) = ms1.(initial_st).
+  (* Global Instance refs: RefStrong _t := *)
+  (*   fun ms0 ms1 => Forall2 (fun '(fn0, ktr0) '(fn1, ktr1) => fn0 = fn1 /\ *)
+  (*                      (forall x, simg (fun _ _ => eq) 0 0 (ktr0 x) (ktr1 x))) *)
+  (*                    ms0.(fnsems) ms1.(fnsems) *)
+  (*                  /\ ms0.(initial_st) = ms1.(initial_st). *)
 
   Lemma core_idemp: forall ms0, | |ms0| | ≡ |ms0|.
   Proof.
